

$$(a.1) \quad m(x) = \frac{1}{N} \sum_{i=1}^N x_i$$

$$y_i = a + bx_i$$

$$m(a + bx) = \frac{1}{N} \sum_{i=1}^N (a + bx_i)$$

Split using rules of summation:

$$m(a + bx) = \frac{1}{N} \left(\sum_{i=1}^N a + \sum_{i=1}^N bx_i \right)$$

$\sum a = Na$ so leave constant b out:

$$m(a + bx) = \frac{Na}{N} + b \left(\frac{1}{N} \sum x_i \right)$$

Substitute definition of $m(x)$:

$$m(a + bx) = a + b \cdot m(x)$$

$$(6.2) \text{ cov}(x, y) = \frac{1}{N} \sum_{i=1}^N (x_i - m(x))(y_i - m(y))$$

$$s^2 = \frac{1}{N} \sum_{i=1}^N (x_i - m(x))^2$$

plug in x for y for covariance formula:

$$\text{cov}(x, x) = \frac{1}{N} \sum_{i=1}^N (x_i - m(x))(x_i - m(x))$$

$$\text{cov}(x, x) = \frac{1}{N} \sum_{i=1}^N (x_i - m(x))^2$$

This is the same as the formula
for s^2

$$6.3) \quad m(a + bY) = a + b \cdot m(Y)$$

$$\text{cov}(x, a + bY) = \frac{1}{N} \sum (x_i - m(x))([a + by_i] - m(a + bY))$$

substitute $m(a + bY)$ with $a + b \cdot m(Y)$:

$$\text{cov}(x, a + bY) = \frac{1}{N} \sum (x_i - m(x))(a + by_i - a - b \cdot m(Y))$$

A terms cancel out:

$$\text{cov}(x, a + bY) = \frac{1}{N} \sum (x_i - m(x))(b(y_i - m(Y)))$$

b goes out:

$$\text{cov}(x, a + bY) = b \cdot \text{cov}(x, Y)$$

6.4) Substitute, so constants a
cancel out and b factors out

$$\text{cov}(a+bx, a+by) = \frac{1}{n} \sum (b(x_i - \bar{x})) \cdot b(y_i - \bar{y})$$

factor out b terms:

$$\text{cov}(a+bx, a+by) = b^2 \cdot \text{cov}(x, y)$$

The reason is because in Q 6.2,

$\text{cov}(x, x) = s^2$. Therefore

$$\text{cov}(bx, bx) = b^2 s^2$$

6.5) $x_1, x_2, x_3, \dots, x_N$

$$y_i = a + bx_i$$

Since $b > 0$, the transformation is increasing. The order stays the same. Additionally, the middle values of y come from the middle values of x .

So if the median of x is $\text{med}(x)$, the median of y is $\text{med}(y) = a + b\text{med}(x)$. Therefore, we can conclude that:

$$\text{med}(a + bx) = a + b\text{med}(x).$$

So, the median of $a + bx$ equals to $a + b\text{med}(x)$.

$$\text{IQR}(x) = Q_3(x) - Q_1(x)$$

Quantiles transform the same way.

$$Q_1(y) = a + bQ_1(x) \quad Q_3(y) = a + bQ_3(x)$$

$$\begin{aligned} \text{IQR}(y) &= Q_3(y) - Q_1(y) \\ &= (a + bQ_3(x)) - (a + bQ_1(x)) \\ &= b(Q_3(x) - Q_1(x)) = b\text{IQR}(x) \end{aligned}$$

So it's true that $\text{IQR}(a + bx) = b\text{IQR}(x)$.

However, it is not true that $\text{IQR}(a + bx)$ is equal to $a + b\text{IQR}(x)$.

6.4)

Data:

$$x = \{1, 7\}, N = 2$$

Mean of x :

$$m(x) = \frac{1+7}{2} = 4$$

Mean of x^2 :

$$m(x^2) = \frac{1^2 + 7^2}{2} = \frac{1+49}{2} = 25$$

Square of the mean:

$$(m(x))^2 = 4^2 = 16$$

$$25 \neq 16$$

Mean of \sqrt{x} :

$$m(\sqrt{x}) = \frac{\sqrt{1} + \sqrt{7}}{2} = \frac{1 + 2.646}{2} = 1.823$$

Square root of the mean:

$$\sqrt{m(x)} = \sqrt{4} = 2$$

$$1.823 \neq 2$$

Therefore:

$$m(x^2) \neq (m(x))^2 \text{ and } m(\sqrt{x}) \neq \sqrt{m(x)}$$